Lean4Lean/Experimental/Stronger.lean
@@ -1,0 +1,625 @@
+import Lean4Lean.Theory.Typing.Lemmas
+
+namespace Lean4Lean
+
+open VExpr
+
+structure VEnv'.VConstant extends Lean4Lean.VConstant where
+  level : VLevel
+
+structure VEnv'.VDefEq extends Lean4Lean.VDefEq where
+  level : VLevel
+
+@[ext] structure VEnv' where
+  constants : Name → Option (Option VEnv'.VConstant)
+  defeqs : VEnv'.VDefEq → Prop
+
+namespace VEnv'
+
+def empty : VEnv' where
+  constants _ := none
+  defeqs _ := False
+
+instance : EmptyCollection VEnv' := ⟨.empty⟩
+
+protected def out (env : VEnv') : VEnv where
+  constants c := (env.constants c).map (·.map (·.toVConstant))
+  defeqs df := ∃ df', env.defeqs df' ∧ df = df'.toVDefEq
+
+@[simp] theorem empty_out : (∅ : VEnv').out = ∅ := by
+  simp [VEnv'.out, EmptyCollection.emptyCollection, empty, VEnv.empty]
+
+protected structure LE (env1 env2 : VEnv') : Prop where
+  constants : env1.constants n = some a → env2.constants n = some a
+  defeqs : env1.defeqs df → env2.defeqs df
+
+instance : LE VEnv' := ⟨VEnv'.LE⟩
+
+theorem LE.rfl {env : VEnv'} : env ≤ env := ⟨id, id⟩
+
+theorem LE.trans {a b c : VEnv'} (h1 : a ≤ b) (h2 : b ≤ c) : a ≤ c :=
+  ⟨h2.1 ∘ h1.1, h2.2 ∘ h1.2⟩
+
+section
+set_option hygiene false
+local notation:65 Γ " ⊢ " e " : " A:30 " : " l:30 => IsDefEqStrong Γ e e A l
+local notation:65 Γ " ⊢ " e1 " ≡ " e2 " : " A:30 " : " l:30 => IsDefEqStrong Γ e1 e2 A l
+variable (env : VEnv') (uvars : Nat)
+
+abbrev VCtx := List (VExpr × VLevel)
+
+def VCtx.out : VCtx → List VExpr := List.map Prod.fst
+
+inductive Lookup : VCtx → Nat → VExpr → VLevel → Prop where
+  | zero : Lookup ((ty, u)::Γ) 0 ty.lift u
+  | succ : Lookup Γ n ty u → Lookup ((A, v)::Γ) (n+1) ty.lift u
+
+inductive IsDefEqStrong : VCtx → VExpr → VExpr → VExpr → VLevel → Prop where
+  | bvar : Lookup Γ i A u → u.WF uvars → Γ ⊢ A : .sort u : .succ u → Γ ⊢ .bvar i : A : u
+  | symm : Γ ⊢ e ≡ e' : A : u → Γ ⊢ e' ≡ e : A : u
+  | trans : Γ ⊢ e₁ ≡ e₂ : A : u → Γ ⊢ e₂ ≡ e₃ : A : u → Γ ⊢ e₁ ≡ e₃ : A : u
+  | sortDF :
+    l.WF uvars → l'.WF uvars → l ≈ l' →
+    Γ ⊢ .sort l ≡ .sort l' : .sort (.succ l) : .succ (.succ l)
+  | constDF :
+    env.constants c = some (some ci) →
+    (∀ l ∈ ls, l.WF uvars) →
+    (∀ l ∈ ls', l.WF uvars) →
+    ls.length = ci.uvars →
+    List.Forall₂ (· ≈ ·) ls ls' →
+    u ≈ ci.level.inst ls → u.WF uvars →
+    [] ⊢ ci.type.instL ls : .sort u : .succ u →
+    [] ⊢ ci.type.instL ls' : .sort u : .succ u →
+    Γ ⊢ ci.type.instL ls : .sort u : .succ u →
+    Γ ⊢ ci.type.instL ls' : .sort u : .succ u →
+    Γ ⊢ .const c ls ≡ .const c ls' : ci.type.instL ls : u
+  | appDF :
+    u.WF uvars → v.WF uvars →
+    Γ ⊢ A : .sort u : .succ u →
+    (A,u)::Γ ⊢ B : .sort v : .succ v →
+    Γ ⊢ f ≡ f' : .forallE A B : .imax u v →
+    Γ ⊢ a ≡ a' : A : u →
+    Γ ⊢ B.inst a ≡ B.inst a' : .sort v : .succ v →
+    Γ ⊢ .app f a ≡ .app f' a' : B.inst a : v
+  | lamDF :
+    u.WF uvars → v.WF uvars →
+    Γ ⊢ A ≡ A' : .sort u : .succ u →
+    (A, u)::Γ ⊢ B : .sort v : .succ v →
+    (A', u)::Γ ⊢ B : .sort v : .succ v →
+    (A, u)::Γ ⊢ body ≡ body' : B : v →
+    (A', u)::Γ ⊢ body ≡ body' : B : v →
+    Γ ⊢ .lam A body ≡ .lam A' body' : .forallE A B : .imax u v
+  | forallEDF :
+    u.WF uvars → v.WF uvars →
+    Γ ⊢ A ≡ A' : .sort u : .succ u →
+    (A, u)::Γ ⊢ body ≡ body' : .sort v : .succ v →
+    (A', u)::Γ ⊢ body ≡ body' : .sort v : .succ v →
+    Γ ⊢ .forallE A body ≡ .forallE A' body' : .sort (.imax u v) : .succ (.imax u v)
+  | defeqDF :
+    u.WF uvars → Γ ⊢ A ≡ B : .sort u : .succ u → Γ ⊢ e1 ≡ e2 : A : u → Γ ⊢ e1 ≡ e2 : B : u
+  | defeqL :
+    u.WF uvars → v.WF uvars → u ≈ v → Γ ⊢ e1 ≡ e2 : A : u → Γ ⊢ e1 ≡ e2 : A : v
+  | beta :
+    u.WF uvars → v.WF uvars → Γ ⊢ A : .sort u : .succ u → (A, u)::Γ ⊢ B : .sort v : .succ v →
+    (A, u)::Γ ⊢ e : B : v → Γ ⊢ e' : A : u →
+    Γ ⊢ B.inst e' : .sort v : .succ v →
+    Γ ⊢ e.inst e' : B.inst e' : v →
+    Γ ⊢ .app (.lam A e) e' ≡ e.inst e' : B.inst e' : v
+  | eta :
+    u.WF uvars → v.WF uvars →
+    Γ ⊢ A : .sort u : .succ u →
+    (A, u)::Γ ⊢ B : .sort v : .succ v →
+    (A.lift, u)::(A, u)::Γ ⊢ B.liftN 1 1 : .sort v : .succ v →
+    Γ ⊢ e : .forallE A B : .imax u v →
+    (A, u)::Γ ⊢ e.lift : .forallE A.lift (B.liftN 1 1) : .imax u v →
+    Γ ⊢ .lam A (.app e.lift (.bvar 0)) ≡ e : .forallE A B : .imax u v
+  | proofIrrel :
+    Γ ⊢ p : .sort .zero : .succ .zero → Γ ⊢ h : p : .zero → Γ ⊢ h' : p : .zero →
+    Γ ⊢ h ≡ h' : p : .zero
+  | extra :
+    env.defeqs df → (∀ l ∈ ls, l.WF uvars) → ls.length = df.uvars →
+    u ≈ df.level.inst ls → u.WF uvars →
+    [] ⊢ df.type.instL ls : .sort u : .succ u →
+    [] ⊢ df.lhs.instL ls : df.type.instL ls : u →
+    [] ⊢ df.rhs.instL ls : df.type.instL ls : u →
+    Γ ⊢ df.lhs.instL ls : df.type.instL ls : u →
+    Γ ⊢ df.rhs.instL ls : df.type.instL ls : u →
+    Γ ⊢ df.lhs.instL ls ≡ df.rhs.instL ls : df.type.instL ls : u
+
+end
+
+def HasType (env : VEnv') (U : Nat) (Γ : VCtx) (e A : VExpr) (u : VLevel) : Prop :=
+  IsDefEqStrong env U Γ e e A u
+
+def IsType (env : VEnv') (U : Nat) (Γ : VCtx) (A : VExpr) (u : VLevel) : Prop :=
+  env.HasType U Γ A (.sort u) (.succ u)
+
+def VConstant.WF (env : VEnv') (ci : VConstant) : Prop := env.IsType ci.uvars [] ci.type ci.level
+
+def VDefEq.WF (env : VEnv') (df : VDefEq) : Prop :=
+  env.HasType df.uvars [] df.lhs df.type df.level ∧ env.HasType df.uvars [] df.rhs df.type df.level
+
+def addConst (env : VEnv') (name : Name) (ci : Option VConstant) : Option VEnv' :=
+  match env.constants name with
+  | some _ => none
+  | none => some { env with constants := fun n => if name = n then some ci else env.constants n }
+
+theorem addConst_out {env : VEnv'} (H : env.addConst n ci = some env₂) :
+    env.out.addConst n (ci.map (·.toVConstant)) = some env₂.out := by
+  revert H; simp [addConst, VEnv.addConst, VEnv'.out]
+  cases env.constants n <;> simp
+  rintro rfl; simp; ext x; split <;> simp
+
+theorem constants_out {env : VEnv'} (H : env.constants n = some (some ci)) :
+    env.out.constants n = some (some ci.toVConstant) := by simp [VEnv'.out, H]
+
+theorem defeqs_out {env : VEnv'} (H : env.defeqs df) :
+    env.out.defeqs df.toVDefEq := ⟨_, H, rfl⟩
+
+def addDefEq (env : VEnv') (df : VDefEq) : VEnv' :=
+  { env with defeqs := fun x => x = df ∨ env.defeqs x }
+
+@[simp] theorem addDefEq_out {env : VEnv'} :
+    (env.addDefEq df).out = env.out.addDefEq df.toVDefEq := by
+  simp [VEnv'.out, addDefEq, VEnv.addDefEq]
+
+theorem IsDefEqStrong.hasType {env : VEnv'}
+    (H : env.IsDefEqStrong U Γ e1 e2 A u) :
+    env.IsDefEqStrong U Γ e1 e1 A u ∧ env.IsDefEqStrong U Γ e2 e2 A u :=
+  ⟨H.trans H.symm, H.symm.trans H⟩
+
+inductive Ctx.LiftN (n : Nat) : Nat → VCtx → VCtx → Prop where
+  | zero (As : VCtx) (h : As.length = n := by rfl) : Ctx.LiftN n 0 Γ (As ++ Γ)
+  | succ : Ctx.LiftN n k Γ Γ' → Ctx.LiftN n (k+1) ((A, u)::Γ) ((A.liftN n k, u) :: Γ')
+
+theorem Lookup.weakN (W : Ctx.LiftN n k Γ Γ') (H : Lookup Γ i A u) :
+    Lookup Γ' (liftVar n i k) (A.liftN n k) u := by
+  induction W generalizing i A u with
+  | zero As =>
+    rw [liftVar_base, Nat.add_comm]
+    subst n
+    induction As with simp [*]
+    | cons _ _ ih => rw [liftN_succ]; exact .succ ih
+  | @succ k _ _ _ _ _ ih =>
+    match H with
+    | .zero => rw [liftVar_zero, ← lift_liftN']; exact .zero
+    | .succ H => rw [liftVar_succ, ← lift_liftN']; exact (ih H).succ
+
+theorem Lookup.out (H : Lookup Γ n ty u) : Lean4Lean.Lookup Γ.out n ty := by
+  induction H with
+  | zero => exact .zero
+  | succ _ ih => exact .succ ih
+
+theorem IsDefEqStrong.out
+    (H : IsDefEqStrong env U Γ e1 e2 A u) : env.out.IsDefEq U Γ.out e1 e2 A := by
+  induction H with
+  | bvar h => exact .bvar h.out
+  | symm _ ih => exact .symm ih
+  | trans _ _ ih1 ih2 => exact .trans ih1 ih2
+  | sortDF h1 h2 h3 => exact .sortDF h1 h2 h3
+  | constDF h1 h2 h3 h4 h5 => exact .constDF (constants_out h1) h2 h3 h4 h5
+  | appDF _ _ _ _ _ _ _ _ _ ih1 ih2 => exact .appDF ih1 ih2
+  | lamDF _ _ _ _ _ _ _ ih1 _ _ ih2 => exact .lamDF ih1 ih2
+  | forallEDF _ _ _ _ _ ih1 ih2 => exact .forallEDF ih1 ih2
+  | defeqDF _ _ _ ih1 ih2 => exact .defeqDF ih1 ih2
+  | defeqL _ _ _ _ ih => exact ih
+  | beta _ _ _ _ _ _ _ _ _ _ ih1 ih2 => exact .beta ih1 ih2
+  | eta _ _ _ _ _ _ _ _ _ _ ih => exact .eta ih
+  | proofIrrel _ _ _ ih1 ih2 ih3 => exact .proofIrrel ih1 ih2 ih3
+  | extra h1 h2 h3 => exact .extra (defeqs_out h1) h2 h3
+
+nonrec theorem HasType.out (H : HasType env U Γ e A u) : env.out.HasType U Γ.out e A := H.out
+
+nonrec theorem IsType.out (H : IsType env U Γ A u) : env.out.IsType U Γ.out A :=
+  ⟨_, H.out⟩
+
+nonrec theorem VConstant.WF.out {ci : VConstant} (H : ci.WF env) : ci.toVConstant.WF env.out :=
+  H.out
+
+theorem VDefEq.WF.out {ci : VDefEq} (H : ci.WF env) : ci.toVDefEq.WF env.out :=
+  ⟨H.1.out, H.2.out⟩
+
+inductive Ordered : VEnv' → Prop where
+  | empty : Ordered ∅
+  | const :
+    Ordered env → (∀ ci, oci = some ci → ci.WF env) →
+    env.addConst n oci = some env' → Ordered env'
+  | defeq : Ordered env → df.WF env → Ordered (env.addDefEq df)
+
+theorem Ordered.out (H : Ordered env) : env.out.Ordered := by
+  induction H with
+  | empty => simp; exact .empty
+  | const h1 h2 h3 ih => exact .const ih (by simp; exact fun _ h => (h2 _ h).out) (addConst_out h3)
+  | defeq h1 h2 ih => exact addDefEq_out ▸ .defeq ih h2.out
+
+def OnTypes (env : VEnv') (P : Nat → VExpr → VExpr → VLevel → Prop) : Prop :=
+  (∀ {n ci}, env.constants n = some (some ci) →
+    P ci.uvars ci.type (.sort ci.level) (.succ ci.level)) ∧
+  (∀ {df}, env.defeqs df → P df.uvars df.lhs df.type df.level ∧ P df.uvars df.rhs df.type df.level)
+
+variable! (henv : Ordered env) in
+theorem IsDefEqStrong.weakN (W : Ctx.LiftN n k Γ Γ') (H : env.IsDefEqStrong U Γ e1 e2 A u) :
+    env.IsDefEqStrong U Γ' (e1.liftN n k) (e2.liftN n k) (A.liftN n k) u := by
+  induction H generalizing k Γ' with
+  | bvar h1 h2 _ ih3 => refine .bvar (h1.weakN W) h2 (ih3 W)
+  | symm _ ih => exact .symm (ih W)
+  | trans _ _ ih1 ih2 => exact .trans (ih1 W) (ih2 W)
+  | sortDF h1 h2 h3 => exact .sortDF h1 h2 h3
+  | constDF h1 h2 h3 h4 h5 h6 h7 h8 h9 _ _ _ _ ih3 ih4 =>
+    simp [(henv.out.closedC (constants_out h1)).instL.liftN_eq (Nat.zero_le _)] at ih3 ih4 ⊢
+    exact .constDF h1 h2 h3 h4 h5 h6 h7 h8 h9 (ih3 W) (ih4 W)
+  | appDF h1 h2 _ _ _ _ _ ih1 ih2 ih3 ih4 ih5 =>
+    refine liftN_inst_hi .. ▸ .appDF h1 h2 (ih1 W) (ih2 W.succ) (ih3 W) (ih4 W) ?_
+    exact liftN_inst_hi .. ▸ liftN_inst_hi .. ▸ ih5 W
+  | lamDF h1 h2 _ _ _ _ _ ih1 ih2 ih3 ih4 ih5 =>
+    exact .lamDF h1 h2 (ih1 W) (ih2 W.succ) (ih3 W.succ) (ih4 W.succ) (ih5 W.succ)
+  | forallEDF h1 h2 _ _ _ ih1 ih2 ih3 => exact .forallEDF h1 h2 (ih1 W) (ih2 W.succ) (ih3 W.succ)
+  | defeqDF h1 _ _ ih1 ih2 => exact .defeqDF h1 (ih1 W) (ih2 W)
+  | defeqL h1 h2 h3 _ ih => exact .defeqL h1 h2 h3 (ih W)
+  | beta h1 h2 _ _ _ _ _ _ ih1 ih2 ih3 ih4 ih5 ih6 =>
+    refine liftN_inst_hi .. ▸ liftN_instN_hi .. ▸ .beta h1 h2
+      (ih1 W) (ih2 W.succ) (ih3 W.succ) (ih4 W)
+      (liftN_instN_hi .. ▸ ih5 W :)
+      (liftN_instN_hi .. ▸ liftN_instN_hi .. ▸ ih6 W :)
+  | @eta Γ a u B v e h1 h2 _ _ _ _ _ ih1 ih2 ih3 ih4 ih5 =>
+    have := IsDefEqStrong.eta h1 h2 (ih1 W) (ih2 W.succ) ?_ (ih4 W) ?_
+    · simp [liftN]; rwa [← lift_liftN']
+    · specialize ih3 W.succ.succ
+      have := liftN'_comm B n 1 (k+1) 1 (Nat.le_add_left ..)
+      rw [Nat.add_comm 1] at this; rwa [← this, ← lift_liftN'] at ih3
+    · have ih5 : IsDefEqStrong _ _ _ _ _ (liftN n (lift (forallE ..)) _) _ := ih5 W.succ
+      rwa [← lift_liftN', ← lift_liftN'] at ih5
+  | proofIrrel _ _ _ ih1 ih2 ih3 => exact .proofIrrel (ih1 W) (ih2 W) (ih3 W)
+  | extra h1 h2 h3 h4 h5 h6 h7 h8 _ _ _ _ _ ih4 ih5 =>
+    have ⟨⟨hA1, _⟩, hA2, hA3⟩ := henv.out.closed.2 (defeqs_out h1)
+    simp [
+      hA1.instL.liftN_eq (Nat.zero_le _),
+      hA2.instL.liftN_eq (Nat.zero_le _),
+      hA3.instL.liftN_eq (Nat.zero_le _)] at ih4 ih5 ⊢
+    exact IsDefEqStrong.extra h1 h2 h3 h4 h5 h6 h7 h8 (ih4 W) (ih5 W)
+
+variable! {env env' : VEnv'} (henv : env ≤ env') in
+theorem IsDefEqStrong.mono
+    (H : env.IsDefEqStrong U Γ e1 e2 A u) : env'.IsDefEqStrong U Γ e1 e2 A u := by
+  induction H with
+  | bvar h1 h2 _ ih => exact .bvar h1 h2 ih
+  | symm _ ih => exact .symm ih
+  | trans _ _ ih1 ih2 => exact .trans ih1 ih2
+  | sortDF h1 h2 h3 => exact .sortDF h1 h2 h3
+  | constDF h1 h2 h3 h4 h5 h6 h7 _ _ _ _ ih1 ih2 ih3 ih4 =>
+    exact .constDF (henv.1 h1) h2 h3 h4 h5 h6 h7 ih1 ih2 ih3 ih4
+  | appDF h1 h2 _ _ _ _ _ ih1 ih2 ih3 ih4 ih5 => exact .appDF h1 h2 ih1 ih2 ih3 ih4 ih5
+  | lamDF h1 h2  _ _ _ _ _ ih1 ih2 ih3 ih4 ih5 => exact .lamDF h1 h2 ih1 ih2 ih3 ih4 ih5
+  | forallEDF h1 h2 _ _ _ ih1 ih2 ih3 => exact .forallEDF h1 h2 ih1 ih2 ih3
+  | defeqDF h1 _ _ ih1 ih2 => exact .defeqDF h1 ih1 ih2
+  | defeqL h1 h2 h3 _ ih => exact .defeqL h1 h2 h3 ih
+  | beta h1 h2 _ _ _ _ _ _ ih1 ih2 ih3 ih4 ih5 ih6 => exact .beta h1 h2 ih1 ih2 ih3 ih4 ih5 ih6
+  | eta h1 h2 _ _ _ _ _ ih1 ih2 ih3 ih4 ih5 => exact .eta h1 h2 ih1 ih2 ih3 ih4 ih5
+  | proofIrrel _ _ _ ih1 ih2 ih3 => exact .proofIrrel ih1 ih2 ih3
+  | extra h1 h2 h3 h4 h5 _ _ _ _ _ ih1 ih2 ih3 ih4 ih5 =>
+    exact .extra (henv.2 h1) h2 h3 h4 h5 ih1 ih2 ih3 ih4 ih5
+
+variable! (henv : Ordered env) in
+theorem IsDefEqStrong.weak0 (H : env.IsDefEqStrong U [] e1 e2 A u) :
+    env.IsDefEqStrong U Γ e1 e2 A u := by
+  have ⟨h1, h2, h3⟩ := H.out.closedN' henv.out.closed ⟨⟩
+  simpa [h1.liftN_eq (Nat.zero_le _), h2.liftN_eq (Nat.zero_le _),
+    h3.liftN_eq (Nat.zero_le _)] using H.weakN henv (.zero Γ rfl)
+
+def VCtx.instL (ls : List VLevel) : VCtx → VCtx := List.map fun (A, u) => (A.instL ls, u.inst ls)
+
+theorem Lookup.instL : Lookup Γ i A u → Lookup (Γ.instL ls) i (A.instL ls) (u.inst ls)
+  | .zero => instL_liftN ▸ .zero
+  | .succ h => instL_liftN ▸ .succ h.instL
+
+variable! {env : VEnv'} {ls : List VLevel} (hls : ∀ l ∈ ls, l.WF U') in
+theorem IsDefEqStrong.instL (H : env.IsDefEqStrong U Γ e1 e2 A u) :
+    env.IsDefEqStrong U' (Γ.instL ls) (e1.instL ls) (e2.instL ls) (A.instL ls) (u.inst ls) := by
+  induction H with
+  | bvar h _ _ ih =>
+    exact .bvar h.instL (.inst hls) ih
+  | constDF h1 h2 h3 h4 h5 h6 _ _ _ _ _ ih1 ih2 ih3 ih4 =>
+    simp [VExpr.instL, VExpr.instL_instL] at ih1 ih2 ih3 ih4 ⊢
+    exact .constDF h1
+      (by simp [VLevel.WF.inst hls]) (by simp [VLevel.WF.inst hls]) (by simp [h4])
+      (by simpa using h5.imp fun _ _ => VLevel.inst_congr_l)
+      (VLevel.inst_inst ▸ VLevel.inst_congr_l h6) (.inst hls) ih1 ih2 ih3 ih4
+  | symm _ ih => exact .symm ih
+  | trans _ _ ih1 ih2 => exact .trans ih1 ih2
+  | sortDF _ _ h3 =>
+    exact .sortDF (VLevel.WF.inst hls) (VLevel.WF.inst hls) (VLevel.inst_congr_l h3)
+  | appDF _ _ _ _ _ _ _ ih1 ih2 ih3 ih4 ih5 =>
+    exact instL_instN ▸ .appDF (.inst hls) (.inst hls)
+      ih1 ih2 ih3 ih4 (instL_instN ▸ instL_instN ▸ ih5)
+  | lamDF _ _ _ _ _ _ _ ih1 ih2 ih3 ih4 ih5 =>
+    exact .lamDF (.inst hls) (.inst hls) ih1 ih2 ih3 ih4 ih5
+  | forallEDF _ _ _ _ _ ih1 ih2 ih3 =>
+    exact .forallEDF (.inst hls) (.inst hls) ih1 ih2 ih3
+  | defeqDF _ _ _ ih1 ih2 => exact .defeqDF (.inst hls) ih1 ih2
+  | defeqL _ _ h3 _ ih => exact .defeqL (.inst hls) (.inst hls) (VLevel.inst_congr_l h3) ih
+  | beta _ _ _ _ _ _ _ _ ih1 ih2 ih3 ih4 ih5 ih6 =>
+    simpa using .beta (.inst hls) (.inst hls) ih1 ih2 ih3 ih4
+      (by simpa using ih5) (by simpa using ih6)
+  | eta _ _ _ _ _ _ _ ih1 ih2 ih3 ih4 ih5 =>
+    simpa [VExpr.instL] using .eta (.inst hls) (.inst hls) ih1 ih2
+      (by simpa [VCtx.instL] using ih3) ih4 (by simpa [VExpr.instL] using ih5)
+  | proofIrrel _ _ _ ih1 ih2 ih3 =>
+    exact .proofIrrel ih1 ih2 ih3
+  | extra h1 h2 h3 h4 _ _ _ _ _ _ ih1 ih2 ih3 ih4 ih5 =>
+    simp [VExpr.instL, VExpr.instL_instL] at ih1 ih2 ih3 ih4 ih5 ⊢
+    exact .extra h1 (by simp [VLevel.WF.inst hls]) (by simp [h3])
+      (VLevel.inst_inst ▸ VLevel.inst_congr_l h4) (.inst hls) ih1 ih2 ih3 ih4 ih5
+
+def VCtx.On (Γ : VCtx) (P : VCtx → VExpr → VLevel → Prop) : Prop :=
+  match Γ with
+  | [] => True
+  | (A, u)::Γ => On Γ P ∧ P Γ A u
+
+def CtxStrong (env : VEnv') (U) (Γ : VCtx) :=
+  Γ.On fun Γ A u => env.IsDefEqStrong U Γ A A (.sort u) (.succ u)
+
+theorem VCtx.On.lookup (h : On Γ P) (hL : Lookup Γ n A u)
+    (hP : ∀ {Γ A B u}, P Γ A u → P (B::Γ) A.lift u) : P Γ A u :=
+  match hL, h with
+  | .zero, ⟨h1, h2⟩ => hP h2
+  | .succ hL, ⟨h1, h2⟩ => hP (h1.lookup hL hP)
+
+variable! (henv : Ordered env) in
+nonrec theorem CtxStrong.lookup {Γ} (H : CtxStrong env U Γ) (h : Lookup Γ i A u) :
+    env.IsDefEqStrong U Γ A A (.sort u) (.succ u) :=
+  H.lookup h fun h => h.weakN henv (.zero [_])
+
+theorem VCtx.On.mono (H : ∀ {Γ A u}, P Γ A u → Q Γ A u) : ∀ {Γ}, On Γ P → On Γ Q
+  | [], h => h
+  | _::_, ⟨h1, h2⟩ => ⟨mono H h1, H h2⟩
+
+theorem CtxStrong.out : ∀ {Γ}, CtxStrong env U Γ → OnCtx Γ.out (env.out.IsType U)
+  | [], h => h
+  | _::_, ⟨h1, h2⟩ => ⟨out h1, _, h2.out⟩
+
+variable (Γ₀ : VCtx) (e₀ A₀ : VExpr) (u₀ : VLevel) in
+inductive Ctx.InstN' : Nat → VCtx → VCtx → Prop where
+  | zero : Ctx.InstN' 0 ((A₀, u₀) :: Γ₀) Γ₀
+  | succ : Ctx.InstN' k Γ Γ' → Ctx.InstN' (k+1) ((A, u)::Γ) ((A.inst e₀ k, u) :: Γ')
+
+variable! (henv : Ordered env) (h₀ : env.IsDefEqStrong U Γ₀ e₀ e₀ A₀ u₀)
+  (hΓ₀ : CtxStrong env U Γ₀) in
+theorem IsDefEqStrong.instN (W : Ctx.InstN' Γ₀ e₀ A₀ u₀ k Γ₁ Γ)
+    (H : env.IsDefEqStrong U Γ₁ e1 e2 A u) (hΓ : CtxStrong env U Γ) :
+    env.IsDefEqStrong U Γ (e1.inst e₀ k) (e2.inst e₀ k) (A.inst e₀ k) u := by
+  induction H generalizing Γ k with
+  | @bvar _ i ty _ h _ h2 ih =>
+    dsimp [inst]; clear h2 ih
+    induction W generalizing i ty with
+    | zero =>
+      cases h with simp [inst_lift]
+      | zero => exact h₀
+      | succ h =>
+        have hty := hΓ₀.lookup henv h
+        exact .bvar h (hty.out.sort_r henv.out hΓ₀.out) hty
+    | succ _ ih =>
+      cases h with (simp; rw [Nat.add_comm, ← liftN_instN_lo (hj := Nat.zero_le _)])
+      | zero =>
+        have hty := hΓ.lookup henv .zero
+        exact .bvar .zero (hty.out.sort_r henv.out hΓ.out) hty
+      | succ h => exact (ih h hΓ.1).weakN henv (.zero [_])
+  | symm _ ih => exact .symm (ih W hΓ)
+  | trans _ _ ih1 ih2 => exact .trans (ih1 W hΓ) (ih2 W hΓ)
+  | sortDF h1 h2 h3 => exact .sortDF h1 h2 h3
+  | constDF h1 h2 h3 h4 h5 h6 h7 h8 h9 _ _ _ _ ih3 ih4 =>
+    simp [(henv.out.closedC (constants_out h1)).instL.instN_eq (Nat.zero_le _)] at ih3 ih4 ⊢
+    exact .constDF h1 h2 h3 h4 h5 h6 h7 h8 h9 (ih3 W hΓ) (ih4 W hΓ)
+  | appDF h1 h2 _ _ _ _ _ ih1 ih2 ih3 ih4 ih5 =>
+    exact inst0_inst_hi .. ▸ .appDF h1 h2
+      (ih1 W hΓ) (ih2 W.succ ⟨hΓ, ih1 W hΓ⟩)
+      (ih3 W hΓ) (ih4 W hΓ) (inst0_inst_hi .. ▸ inst0_inst_hi .. ▸ ih5 W hΓ)
+  | lamDF h1 h2 _ _ _ _ _ ih1 ih2 ih3 ih4 ih5 =>
+    exact
+      have hΓ' := ⟨hΓ, (ih1 W hΓ).hasType.1⟩
+      have hΓ'' := ⟨hΓ, (ih1 W hΓ).hasType.2⟩
+      .lamDF h1 h2 (ih1 W hΓ) (ih2 W.succ hΓ') (ih3 W.succ hΓ'') (ih4 W.succ hΓ') (ih5 W.succ hΓ'')
+  | forallEDF h1 h2 _ _ _ ih1 ih2 ih3 =>
+    exact .forallEDF h1 h2 (ih1 W hΓ)
+      (ih2 W.succ ⟨hΓ, (ih1 W hΓ).hasType.1⟩) (ih3 W.succ ⟨hΓ, (ih1 W hΓ).hasType.2⟩)
+  | defeqDF h1 _ _ ih1 ih2 => exact .defeqDF h1 (ih1 W hΓ) (ih2 W hΓ)
+  | defeqL h1 h2 h3 _ ih => exact .defeqL h1 h2 h3 (ih W hΓ)
+  | beta h1 h2 _ _ _ _ _ _ ih1 ih2 ih3 ih4 ih5 ih6 =>
+    rw [inst0_inst_hi, inst0_inst_hi]; exact
+      have hΓ' := ⟨hΓ, ih1 W hΓ⟩
+      .beta h1 h2
+        (ih1 W hΓ) (ih2 W.succ hΓ') (ih3 W.succ hΓ') (ih4 W hΓ)
+        (inst0_inst_hi .. ▸ ih5 W hΓ) (inst0_inst_hi .. ▸ inst0_inst_hi .. ▸ ih6 W hΓ)
+  | eta h1 h2 _ _ _ _ _ ih1 ih2 ih3 ih4 ih5 =>
+    have :=
+      have hΓ' := ⟨hΓ, (ih1 W hΓ).hasType.1⟩
+      IsDefEqStrong.eta h1 h2 (ih1 W hΓ) (ih2 W.succ hΓ')
+        (by
+          have := ih3 W.succ.succ ⟨hΓ', by
+            rw [← lift_instN_lo]; exact (ih1 W hΓ).hasType.1.weakN henv (.zero [_])⟩
+          rwa [lift_instN_lo, liftN_instN_lo (hj := Nat.le_add_left ..), Nat.add_comm 1])
+        (ih4 W hΓ)
+        (by
+          have := ih5 W.succ hΓ'
+          simp only [inst, ← lift_instN_lo] at this
+          rwa [liftN_instN_lo (hj := Nat.le_add_left ..), Nat.add_comm 1])
+    rw [lift, liftN_instN_lo (hj := Nat.zero_le _), Nat.add_comm] at this
+    simpa [inst]
+  | proofIrrel _ _ _ ih1 ih2 ih3 => exact .proofIrrel (ih1 W hΓ) (ih2 W hΓ) (ih3 W hΓ)
+  | extra h1 h2 h3 h4 h5 h6 h7 h8 _ _ _ _ _ ih4 ih5 =>
+    have ⟨⟨hA1, _⟩, hA2, hA3⟩ := henv.out.closed.2 (defeqs_out h1)
+    simp [
+      hA1.instL.instN_eq (Nat.zero_le _),
+      hA2.instL.instN_eq (Nat.zero_le _),
+      hA3.instL.instN_eq (Nat.zero_le _)] at ih4 ih5 ⊢
+    exact .extra h1 h2 h3 h4 h5 h6 h7 h8 (ih4 W hΓ) (ih5 W hΓ)
+
+theorem IsDefEqStrong.defeqDF_l (henv : Ordered env) (hΓ : CtxStrong env U Γ)
+    (h1 : env.IsDefEqStrong U Γ A A' (.sort u) (.succ u))
+    (h2 : env.IsDefEqStrong U ((A, u)::Γ) e1 e2 B v) :
+    env.IsDefEqStrong U ((A', u)::Γ) e1 e2 B v := by
+  simpa [instN_bvar0] using
+    have hu := h1.out.sort_r henv.out hΓ.out
+    have hΓ' := ⟨hΓ, h1.hasType.2⟩
+    h1.weakN henv (.zero [(A', u)])
+      |>.symm.defeqDF hu (.bvar .zero hu (h1.hasType.2.weakN henv (.zero [(A', u)])))
+      |>.instN henv hΓ' .zero (h2.weakN henv (.succ (.zero [(A', u)]))) hΓ'
+
+def EnvStrong (env : VEnv') (U : Nat) (e A : VExpr) (u : VLevel) : Prop :=
+  env.IsDefEqStrong U [] e e A u ∧
+  env.IsDefEqStrong U [] A A (.sort u) (.succ u) ∧
+  ∀ A B, e = A.forallE B →
+    ∃ u, env.IsDefEqStrong U [] A A (.sort u) (.succ u) ∧
+    ∃ v, env.IsDefEqStrong U [(A, u)] B B (.sort v) (.succ v)
+
+variable! (henv : Ordered env) (envIH : env.OnTypes (EnvStrong env)) in
+theorem IsDefEqStrong.forallE_inv' (hΓ : CtxStrong env U Γ)
+    (H : env.IsDefEqStrong U Γ e1 e2 V v) (eq : e1 = A.forallE B ∨ e2 = A.forallE B) :
+    ∃ u, env.IsDefEqStrong U Γ A A (.sort u) (.succ u) ∧
+    ∃ v, env.IsDefEqStrong U ((A, u)::Γ) B B (.sort v) (.succ v) := by
+  induction H generalizing A B with
+  | symm _ ih => exact ih hΓ eq.symm
+  | trans _ _ ih1 ih2
+  | proofIrrel _ _ _ _ ih1 ih2 =>
+    obtain eq | eq := eq
+    · exact ih1 hΓ (.inl eq)
+    · exact ih2 hΓ (.inr eq)
+  | forallEDF _ _ h1 h2 =>
+    obtain ⟨⟨⟩⟩ | ⟨⟨⟩⟩ := eq
+    · exact ⟨_, h1.hasType.1, _, h2.hasType.1⟩
+    · exact ⟨_, h1.hasType.2, _, h1.defeqDF_l henv hΓ h2.hasType.2⟩
+  | defeqDF _ _ _ _ ih | defeqL _ _ _ _ ih => exact ih hΓ eq
+  | @beta _ _ _ _ _ e _ _ _ h1 _ _ h4 _ _ _ _ ih3 ih4 =>
+    obtain ⟨⟨⟩⟩ | eq := eq
+    cases e with
+    | bvar i =>
+      cases i with simp [inst] at eq
+      | zero => exact ih4 hΓ (.inl eq)
+    | forallE A B =>
+      cases eq
+      let ⟨_, A1, _, A2⟩ := ih3 ⟨hΓ, h1⟩ (.inl rfl)
+      refine ⟨_, h4.instN henv hΓ .zero A1 hΓ, _, h4.instN henv hΓ (.succ .zero) A2 ?_⟩
+      exact ⟨hΓ, h4.instN henv hΓ .zero A1 hΓ⟩
+    | _ => cases eq
+  | eta _ _ _ _ _ _ _ _ _ _ ih =>
+    obtain ⟨⟨⟩⟩ | eq := eq
+    exact ih hΓ (.inl eq)
+  | @extra df ls _ Γ h1 h2 =>
+    suffices ∀ e, VExpr.instL ls e = VExpr.forallE A B →
+        EnvStrong env df.uvars e df.type df.level →
+        ∃ u, IsDefEqStrong env U Γ A A (.sort u) (.succ u) ∧
+        ∃ v, IsDefEqStrong env U ((A, u) :: Γ) B B (.sort v) (.succ v) by
+      have ⟨A1, A2⟩ := envIH.2 h1
+      cases eq <;> exact this _ ‹_› ‹_›
+    intro e eq IH
+    cases e <;> cases eq; rename_i A B
+    let ⟨_, A1, v, A2⟩ := IH.2.2 _ _ rfl
+    refine ⟨_, (A1.instL h2).weak0 henv, v.inst ls, ?_⟩
+    have := (A2.instL h2).weakN henv (.succ (.zero Γ))
+    have C1 := (A1.instL h2).out.closedN henv.out ⟨⟩
+    have C2 := (A2.instL h2).out.closedN henv.out ⟨⟨⟩, C1⟩
+    rw [C1.liftN_eq (Nat.zero_le _), C2.liftN_eq (by exact Nat.le_refl _)] at this
+    simpa [liftN]
+  | _ => nomatch eq
+
+variable! (henv : Ordered env) in
+theorem IsDefEqStrong.isType' (hΓ : CtxStrong env U Γ) (H : env.IsDefEqStrong U Γ e1 e2 A u) :
+    env.IsDefEqStrong U Γ A A (.sort u) (.succ u) := by
+  induction H with
+  | bvar h => exact hΓ.lookup henv h
+  | symm _ ih => exact ih hΓ
+  | trans _ _ ih1 => exact ih1 hΓ
+  | sortDF h1 => exact .sortDF h1 h1 rfl
+  | constDF _ _ _ _ _ _ _ _ _ h => exact h
+  | appDF _ _ _ _ _ _ h4 _ _ _ ih3 => exact h4.hasType.1
+  | lamDF h1 h2 h3 h4 => exact .forallEDF h1 h2 h3.hasType.1 h4 h4
+  | forallEDF h1 h2 => exact .sortDF ⟨h1, h2⟩ ⟨h1, h2⟩ rfl
+  | defeqDF _ h2 => exact h2.hasType.2
+  | defeqL h1 h2 h3 _ ih =>
+    exact (defeqDF (by exact h1) (sortDF h1 h2 h3) (ih hΓ))
+      |>.defeqL (by exact h1) (by exact h2) (VLevel.succ_congr h3)
+  | beta _ _ _ h4 _ h6 => exact h6.hasType.1.instN henv hΓ .zero h4 hΓ
+  | eta _ _ _ _ _ _ _ _ _ _ ih => exact ih hΓ
+  | proofIrrel h1 => exact h1
+  | extra _ _ _ _ _ h => exact h.weak0 henv
+
+theorem IsDefEqStrong.sort_invL {env : VEnv'}
+    (H : env.IsDefEqStrong U Γ e1 e2 A u) :
+    (.sort v = e1 → u ≈ v.succ.succ) ∧
+    (.sort v = e2 → u ≈ v.succ.succ) ∧
+    (.sort v = A → u ≈ v.succ) := by
+  induction H generalizing v with
+  | bvar _ _ _ ih
+  | constDF _ _ _ _ _ _ _ _ _ _ _ _ _ ih
+  | appDF _ _ _ _ _ _ _ _ _ _ _ ih =>
+    exact ⟨nofun, nofun, fun h => VLevel.succ_congr_iff.1 <| ih.1 h⟩
+  | symm _ ih => exact ⟨ih.2.1, ih.1, ih.2.2⟩
+  | trans _ _ ih1 ih2 => exact ⟨ih1.1, ih2.2.1, ih1.2.2⟩
+  | sortDF _ _ h =>
+    refine ⟨by rintro ⟨⟩; rfl, ?_, by rintro ⟨⟩; rfl⟩
+    rintro ⟨⟩; exact VLevel.succ_congr (VLevel.succ_congr h)
+  | lamDF => exact ⟨nofun, nofun, nofun⟩
+  | forallEDF => exact ⟨nofun, nofun, by rintro ⟨⟩; rfl⟩
+  | defeqDF _ _ _ ih1 ih2 => exact ⟨ih2.1, ih2.2.1, fun h => VLevel.succ_congr_iff.1 <| ih1.2.1 h⟩
+  | defeqL _ _ h1 _ ih =>
+    exact ⟨h1.symm.trans ∘ ih.1, h1.symm.trans ∘ ih.2.1, h1.symm.trans ∘ ih.2.2⟩
+  | beta _ _ _ _ _ _ _ _ _ _ _ _ _ ih => exact ⟨nofun, ih.1, ih.2.2⟩
+  | eta _ _ _ _ _ _ _ _ _ _ ih => exact ⟨nofun, ih.1, ih.2.2⟩
+  | proofIrrel _ _ _ _ ih1 ih2
+  | extra _ _ _ _ _ _ _ _ _ _ _ ih1 ih2 => exact ⟨ih1.1, ih2.1, ih1.2.2⟩
+
+variable {env : VEnv'} in
+-- variable! (henv : Ordered env) (hΓ : CtxStrong env U Γ) in
+theorem IsDefEqStrong.uniqL'
+    (H1 : env.IsDefEqStrong U Γ e1 e2 A u)
+    (H2 : env.IsDefEqStrong U Γ e1' e2' A' v)
+    : (e1 = e1' → u ≈ v) ∧ (e1 = e2' → u ≈ v) ∧
+      (e2 = e1' → u ≈ v) ∧ (e2 = e2' → u ≈ v) := by
+  induction H1 generalizing e1' e2' A' v with
+  | bvar H1 h1 h2 ih =>
+    clear h1 h2 ih
+    induction H2 with try simp
+    | @bvar _ _ A' u' H2 h1 h2 ih =>
+      rintro rfl; clear h1 h2 ih
+      induction H1 generalizing A' u' with cases H2
+      | zero => rfl
+      | succ h ih => exact ih ‹_›
+    | symm _ ih => let ⟨h1, h2, h3, h4⟩ := ih H1; exact ⟨h2, h1, h4, h3⟩
+    | trans _ _ ih1 ih2
+    | proofIrrel _ _ _ _ ih1 ih2
+    | extra _ _ _ _ _ _ _ _ _ _ _ _ _ ih1 ih2 =>
+      let ⟨h1, _, h3, _⟩ := ih1 H1; let ⟨_, h2, _, h4⟩ := ih2 H1
+      exact ⟨h1, h2, h3, h4⟩
+    | defeqDF _ _ _ _ ih => exact ih H1
+    | defeqL _ _ h _ ih => exact propext (VLevel.equiv_congr_right h) ▸ ih H1
+    | beta _ _ _ _ _ _ _ _ _ _ _ _ _ ih
+    | eta _ _ _ _ _ _ _ _ _ _ ih => exact (ih H1).1
+  | @constDF c ci ls _ _ _ h1 _ _ _ h2 hu _ d1 d2 d3 d4 ih1 ih2 ih3 ih4 =>
+    clear d1 d2 d3 d4 ih1 ih2 ih3 ih4
+    induction H2 with try simp
+    | @constDF c' _ ls' _ _ _ h1' _ _ _ h2' hu' =>
+      by_cases h : c = c' <;> simp [h]; subst h
+      cases h1.symm.trans h1'
+      rw [VLevel.equiv_congr_left hu, VLevel.equiv_congr_right hu']
+      have eq := VLevel.inst_congr (l := ci.level) rfl h2
+      have eq' := VLevel.inst_congr (l := ci.level) rfl h2'
+      refine ⟨?_, ?_, ?_, ?_⟩ <;> rintro rfl <;>
+        [rfl; exact eq'.symm; exact eq; exact eq.trans eq'.symm]
+    | symm _ ih => let ⟨h1, h2, h3, h4⟩ := ih; exact ⟨h2, h1, h4, h3⟩
+    | trans _ _ ih1 ih2
+    | proofIrrel _ _ _ _ ih1 ih2
+    | extra _ _ _ _ _ _ _ _ _ _ _ _ _ ih1 ih2 =>
+      let ⟨h1, _, h3, _⟩ := ih1; let ⟨_, h2, _, h4⟩ := ih2
+      exact ⟨h1, h2, h3, h4⟩
+    | defeqDF _ _ _ _ ih => exact ih
+    | defeqL _ _ h _ ih => exact propext (VLevel.equiv_congr_right h) ▸ ih
+    | beta _ _ _ _ _ _ _ _ _ _ _ _ _ ih
+    | eta _ _ _ _ _ _ _ _ _ _ ih => exact ⟨ih.1, ih.2.2.1⟩
+  | @appDF _ _ _ _ _ f₁ f₂ a₁ a₂ _ _ d1 d2 d3 d4 d5 ih1 ih2 ih3 ih4 ih5 =>
+    clear d1 d2 d3 d4 d5 ih1 ih2 ih5
+    induction H2 with try simp
+    | @appDF _ _ _ _ _ f₁' f₂' a₁' a₂' _ _ _ _ _ ih3' ih4' =>
+      refine ⟨?_, sorry⟩
+      rintro rfl rfl
+      sorry -- looks like it needs unique typing :(
+    | _ => sorry
+  | _ => sorry
