Lean4Lean/Theory.lean
@@ -1,6 +1,4 @@
 import Lean4Lean.Theory.Typing.EnvLemmas
 import Lean4Lean.Theory.Typing.Strong
-import Lean4Lean.Theory.Typing.Stratified
-import Lean4Lean.Theory.Typing.StratifiedUntyped
 import Lean4Lean.Theory.Typing.ParallelReduction
 import Lean4Lean.Theory.Typing.UniqueTyping
